Code export for renaming preconditions and correctness theorem for renaming

Simple_Networks/Simple_Network_Language_Export_Code.thy
@@ -2,6 +2,139 @@ theory Simple_Network_Language_Export_Code
   imports Simple_Network_Language_Renaming
 begin
 
+datatype result =
+  Renaming_Failed | Preconds_Unsat | Sat | Unsat
+
+abbreviation "renum_automaton \<equiv> Simple_Network_Rename_Defs.renum_automaton"
+
+definition rename_mc where
+  "rename_mc broadcast bounds' automata k L\<^sub>0 s\<^sub>0 formula
+    m num_states num_actions renum_acts renum_vars renum_clocks renum_states
+\<equiv>
+let
+   renaming_valid =
+    Simple_Network_Rename_Formula
+      broadcast bounds' renum_vars renum_clocks renum_states automata formula s\<^sub>0 L\<^sub>0;
+   automata = map_index (renum_automaton renum_acts renum_vars renum_clocks renum_states) automata;
+   broadcast = map renum_acts broadcast;
+   bounds' = map (\<lambda>(a,b,c). (renum_vars a, b, c)) bounds';
+   formula = map_formula renum_states renum_vars id formula;
+   L\<^sub>0 = map_index renum_states L\<^sub>0;
+   s\<^sub>0 = map (\<lambda>(x, v). (renum_vars x, v)) s\<^sub>0
+in
+  if
+    renaming_valid
+  then
+    do {
+    r \<leftarrow> precond_mc broadcast bounds' automata m num_states num_actions k L\<^sub>0 s\<^sub>0 formula;
+    case r of
+      None \<Rightarrow> return Preconds_Unsat
+    | Some False \<Rightarrow> return Unsat
+    | Some True \<Rightarrow> return Sat
+    } 
+  else return Renaming_Failed
+"
+
+theorem model_check_rename:
+  "<emp> rename_mc broadcast bounds automata k L\<^sub>0 s\<^sub>0 formula
+    m num_states num_actions renum_acts renum_vars renum_clocks renum_states
+    <\<lambda> Sat \<Rightarrow> \<up>(
+        (\<not> has_deadlock (N broadcast automata bounds) (L\<^sub>0, map_of s\<^sub>0, \<lambda>_ . 0) \<longrightarrow>
+          N broadcast automata bounds,(L\<^sub>0, map_of s\<^sub>0, \<lambda>_ . 0) \<Turnstile> formula
+        ))
+     | Unsat \<Rightarrow> \<up>(
+        (\<not> has_deadlock (N broadcast automata bounds) (L\<^sub>0, map_of s\<^sub>0, \<lambda>_ . 0) \<longrightarrow>
+          \<not> N broadcast automata bounds,(L\<^sub>0, map_of s\<^sub>0, \<lambda>_ . 0) \<Turnstile> formula
+        ))
+     | Renaming_Failed \<Rightarrow> \<up>(\<not> Simple_Network_Rename_Formula
+        broadcast bounds renum_vars renum_clocks renum_states automata formula s\<^sub>0 L\<^sub>0)
+     | Preconds_Unsat \<Rightarrow> \<up>(\<not> Simple_Network_Impl_nat_ceiling_start_state
+        (map renum_acts broadcast)
+        (map (\<lambda>(a,b,c). (renum_vars a, b, c)) bounds)
+        (map_index (renum_automaton renum_acts renum_vars renum_clocks renum_states) automata)
+        m num_states num_actions k
+        (map_index renum_states L\<^sub>0) (map (\<lambda>(x, v). (renum_vars x, v)) s\<^sub>0)
+        (map_formula renum_states renum_vars id formula))
+    >\<^sub>t"
+proof -
+  define A where "A \<equiv> N broadcast automata bounds"
+  define check where "check \<equiv> A,(L\<^sub>0, map_of s\<^sub>0, \<lambda>_ . 0) \<Turnstile> formula"
+  define A' where "A' \<equiv> N
+    (map renum_acts broadcast)
+    (map_index (renum_automaton renum_acts renum_vars renum_clocks renum_states) automata)
+    (map (\<lambda>(a,b,c). (renum_vars a, b, c)) bounds)
+  "
+  define check' where "check' \<equiv>
+    A',(map_index renum_states L\<^sub>0, map_of (map (\<lambda>(x, v). (renum_vars x, v)) s\<^sub>0), \<lambda>_ . 0) \<Turnstile>
+    map_formula renum_states renum_vars id formula"
+  define preconds_sat where "preconds_sat \<equiv>
+    Simple_Network_Impl_nat_ceiling_start_state
+      (map renum_acts broadcast)
+      (map (\<lambda>(a,b,c). (renum_vars a, b, c)) bounds)
+      (map_index (renum_automaton renum_acts renum_vars renum_clocks renum_states) automata)
+      m num_states num_actions k
+      (map_index renum_states L\<^sub>0) (map (\<lambda>(x, v). (renum_vars x, v)) s\<^sub>0)
+      (map_formula renum_states renum_vars id formula)"
+  define renaming_valid where "renaming_valid \<equiv>
+    Simple_Network_Rename_Formula
+      broadcast bounds renum_vars renum_clocks renum_states automata formula s\<^sub>0 L\<^sub>0
+  "
+  have [simp]: "check \<longleftrightarrow> check'" 
+    if renaming_valid
+    using that unfolding check_def check'_def A_def A'_def renaming_valid_def
+    by (rule Simple_Network_Rename_Formula.models_iff'[symmetric])
+  have test[symmetric, simp]:
+    "Simple_Network_Language_Model_Checking.has_deadlock A (L\<^sub>0, map_of s\<^sub>0, \<lambda>_. 0)
+  \<longleftrightarrow>Simple_Network_Language_Model_Checking.has_deadlock A'
+     (map_index renum_states L\<^sub>0, map_of (map (\<lambda>(x, y). (renum_vars x, y)) s\<^sub>0), \<lambda>_. 0)
+  " if renaming_valid
+    using that unfolding check_def check'_def A_def A'_def renaming_valid_def
+    by (rule Simple_Network_Rename_Formula.has_deadlock_iff'[symmetric])
+  note bla[sep_heap_rules] =
+    model_check[
+    of "map renum_acts broadcast" "map (\<lambda>(a,b,c). (renum_vars a, b, c)) bounds"
+    "map_index (renum_automaton renum_acts renum_vars renum_clocks renum_states) automata"
+    m num_states num_actions k "map_index renum_states L\<^sub>0" "map (\<lambda>(x, v). (renum_vars x, v)) s\<^sub>0"
+    "map_formula renum_states renum_vars id formula",
+    folded A'_def check'_def preconds_sat_def renaming_valid_def,
+    simplified
+    ]
+  show ?thesis
+    unfolding rename_mc_def
+    unfolding
+      A_def[symmetric] check_def[symmetric]
+      preconds_sat_def[symmetric] renaming_valid_def[symmetric]
+    by (sep_auto
+          simp: model_checker.refine[symmetric] pure_def return_cons_rule split: bool.splits
+       )
+qed
+
+
+paragraph \<open>Code Setup for the Model Checker\<close>
+
+lemmas [code] =
+  reachability_checker_def
+  Alw_ev_checker_def
+  leadsto_checker_def
+  model_checker_def[unfolded PR_CONST_def]
+
+lemmas [code] =
+  Prod_TA_Defs.n_ps_def
+  Simple_Network_Impl.n_vs_def
+  Simple_Network_Impl.automaton_of_def
+  Simple_Network_Impl_nat_defs.pairs_by_action_impl_def
+  Simple_Network_Impl_nat_defs.all_actions_from_vec_def
+  Simple_Network_Impl_nat_defs.all_actions_by_state_def
+  Simple_Network_Impl_nat_defs.compute_upds_impl_def
+  Simple_Network_Impl_nat_defs.actions_by_state_def
+  Simple_Network_Impl_nat_defs.check_boundedi_def
+  Simple_Network_Impl_nat_defs.get_commited_def
+  Simple_Network_Impl_nat_defs.make_combs_def
+  Simple_Network_Impl_nat_defs.trans_map_def
+  Simple_Network_Impl_nat_defs.actions_by_state'_def
+  Simple_Network_Impl_nat_defs.bounds_map_def
+  mk_updsi_def
+
 lemma (in Simple_Network_Impl_nat_defs) bounded_s\<^sub>0_iff:
   "bounded bounds (map_of s\<^sub>0) \<longleftrightarrow> bounded (map_of bounds') (map_of s\<^sub>0)"
   unfolding bounds_def snd_conv ..
@@ -17,5 +150,41 @@ lemmas [code_unfold] = bounded_def dom_map_of_conv_image_fst
 export_code Simple_Network_Impl_nat_ceiling_start_state_axioms
 
 export_code precond_mc in SML module_name Test
+
+
+paragraph \<open>Code Setup for Renaming\<close>
+
+lemmas [code] =
+  Simple_Network_Rename_def
+  Simple_Network_Impl.clk_set'_def
+  Simple_Network_Impl.clkp_set'_def
+
+lemmas [code] =
+  Simple_Network_Rename_Defs.renum_automaton_def
+  Simple_Network_Rename_Defs.renum_cconstraint_def
+  Simple_Network_Rename_Defs.map_cconstraint_def
+  Simple_Network_Rename_Defs.renum_reset_def
+  Simple_Network_Rename_Defs.renum_upd_def
+  Simple_Network_Rename_Defs.renum_act_def
+  Simple_Network_Rename_Defs.renum_exp_def
+
+lemma (in Prod_TA_Defs) states_mem_iff:
+  "L \<in> states \<longleftrightarrow> length L = n_ps \<and>
+  (\<forall> i. i < n_ps \<longrightarrow> (\<exists> (l, g, a, r, u, l') \<in> fst (snd (fst (snd A) ! i)). L ! i = l \<or> L ! i = l'))"
+  unfolding states_def trans_def N_def by (auto split: prod.split)
+
+lemmas [code_unfold] =
+  Prod_TA_Defs.states_mem_iff
+  Simple_Network_Impl.var_set_compute
+  Simple_Network_Impl.loc_set_compute
+  setcompr_eq_image
+  Simple_Network_Impl.length_automata_eq_n_ps[symmetric]
+
+lemmas [code] =
+  Simple_Network_Rename_Formula_def
+  Simple_Network_Rename_Formula_axioms_def
+
+
+export_code rename_mc in SML module_name Test
 
 end
